feat: define third projection and prove correct
Define the first third projection and prove that given an interpreter,
the generated compiler behaves identically to the interpreter for all
input programs and program inputs.

Futamura/Projections.lean
@@ -17,12 +17,20 @@ structure Interp {I O : Type} (S T : Lang) where
   /-- Running the interpreter yields the same result as evaluating the source program directly. -/
   correct: ∀ (p : S.Prog I O) (x: I), S.eval p x = T.eval prog (p, x)
 
+/-- The raw program type of an interpreter for `S` in `T`. -/
+abbrev Interp.ProgType (I O : Type) (S T : Lang) :=
+  T.Prog (S.Prog I O × I) O
+
 /-- A compiler from `S` to `T` written in `T`: a `T`-program that takes a source program from `I` to `O` and returns a `T` program from `I` to `O`. -/
 structure Compiler {I O : Type} (S T : Lang) where
   /-- The compiler program.-/
   prog: T.Prog (S.Prog I O) (T.Prog I O)
   /-- Compiling and running a program yileds the same result as evaluating the source program directly. -/
   correct: ∀ (p : S.Prog I O) (x : I), S.eval p x = T.eval (T.eval prog p) x
+
+/-- The raw program type of a compiler from `S` to `T`. -/
+abbrev Compiler.ProgType (I O : Type) (S T : Lang) :=
+  T.Prog (S.Prog I O) (T.Prog I O)
 
 /-- A specializer (partial evaluator) for `T`: a `T`-program that takes a program expecting a static-dynamic pair and a static input, and produces a residual program over just the dynamic input. -/
 structure Mix (T : Lang) where
@@ -58,3 +66,22 @@ def projection2 {I O : Type}
     rw [← mix.correct]
     rw [← mix.correct]
     rw [← Interp.correct]
+
+/-- Third Futamura projection: specializing `mix` on `mix` to yields a compiler generator from any language to the implementaion language of `mix`. -/
+def projection3 {I O : Type}
+    (S T : Lang)
+    (mix : Mix T)
+    : T.Prog (Interp.ProgType I O S T) (Compiler.ProgType I O S T) :=
+  T.eval mix.prog (mix.prog, mix.prog)
+
+/-- Given an interpreter, the generated compiler behaves identically to the interpreter for all input programs and program inputs. -/
+theorem projection3_correct {I O : Type}
+    (S T : Lang)
+    (mix : Mix T)
+    (interp : Interp.ProgType I O S T)
+    (p : S.Prog I O) (x : I) :
+    T.eval interp (p, x) = T.eval (T.eval (T.eval (projection3 S T mix) interp) p) x := by
+  unfold projection3
+  rw [← mix.correct]
+  rw [← mix.correct]
+  rw [← mix.correct]
